{
 "cells": [
  {
   "cell_type": "markdown",
   "metadata": {},
   "source": [
    "# BGL hydrodynamic equation for the pure case\n",
    "\n",
    "The BGL hydrodynamic equations are:\n",
    "$$\n",
    "\\begin{cases}\n",
    "\\partial t \\rho+ \\Re(\\nabla^* f_1)=0,\\\\\n",
    "\\partial t f_1 = -\\frac{1}{2}\\nabla \\rho + (\\mu_1[\\rho] - \\xi|f_1|^2)f_1 + \\nu \\Delta f_1 + \\kappa_1 f_1^* \\nabla f_1 + \\kappa_2 \\nabla^* f_1^2,\n",
    "\\end{cases}\n",
    "$$\n",
    "where $f_1=p_x+ip_y$, $\\nabla = \\partial_x + i \\partial_y$, $\\Delta = \\nabla \\nabla^*$. The coefficients are\n",
    "\n",
    "\n",
    "| Coefficient | Value | \n",
    "| :-: | :-: |\n",
    "| $\\mu$ | $$P_1 - 1 + \\rho_0 \\rho (J_{1, 0} + J_{1, 1})$$ | \n",
    "| $\\xi$ | $$\\frac{\\rho_0^2(J_{1, 2} + J_{1, -1})J_{2, 1}}{\\mu_2}$$ |\n",
    "| $\\nu$ | $$-\\frac{1}{4\\mu_2}$$ |\n",
    "| $\\kappa_1$ | $$\\frac{\\rho_0(J_{1, 2} + J_{1, -1})}{2\\mu_2}$$ |\n",
    "| $\\kappa_2$ | $$\\frac{\\rho_0 J_{2, 1}}{2\\mu_2}$$ |\n",
    "\n",
    "Here $\\mu_2 = P_2 - 1 + \\rho_0 (J_{2, 0} + J_{2, 2})$, $P_k = \\exp (-\\frac{k^2\\eta^2}{2})$, the mode coupling functions $J_{k, q} = P_k I_{k, q} - I_{0, q}$ with\n",
    "\n",
    "$$\n",
    "I_{k, q}=\\begin{cases}\n",
    "\\frac{4}{\\pi}\\frac{1-(k-2q)(-1)^q\\sin (\\frac{k\\pi}{2})}{1-(k-2q)^2}\\quad & \\mathrm{if}\\ |k-2q| \\neq 1,\\\\\n",
    "\\frac{2}{\\pi}\\quad &\\mathrm{otherwise}.\n",
    "\\end{cases}\n",
    "$$\n"
   ]
  },
  {
   "cell_type": "markdown",
   "metadata": {},
   "source": [
    "## Linear term:\n",
    "$$\n",
    "\\begin{cases}\n",
    "\\partial_t \\rho = - (\\partial_x p_x + \\partial_y p_y)\\\\\n",
    "\\partial_t p_x = -\\frac{1}{2} \\partial_x \\rho + \\mu_1 p_x + \\nu (\\partial^2_x + \\partial^2_y) p_x, \\\\\n",
    "\\partial_t p_y = -\\frac{1}{2} \\partial_y \\rho + \\mu_1 p_y + \\nu (\\partial^2_x + \\partial^2_y) p_y,\n",
    "\\end{cases}\n",
    "$$\n",
    "\n",
    "## Nonlinear term:\n",
    "$$\n",
    "\\begin{cases}\n",
    "\\partial_t p_x = (\\mu_\\rho \\rho - \\xi p^2) p_x + \\kappa_1 \\left[p_x (\\partial_x p_x -\\partial_y p_y) + p_y (\\partial_x p_y + \\partial_y p_x)\\right] + 2\\kappa_2 \\left[p_x(\\partial_x p_x + \\partial_y p_y) - p_y (\\partial_x p_y -\\partial_y p_x)\\right],\\\\\n",
    "\\partial_t p_y = (\\mu_\\rho \\rho - \\xi p^2) p_y + \\kappa_1 \\left[p_x (\\partial_x p_y +\\partial_y p_x) - p_y (\\partial_x p_x - \\partial_y p_y)\\right] + 2\\kappa_2 \\left[p_x(\\partial_x p_y - \\partial_y p_x) + p_y (\\partial_x p_x + \\partial_y p_y)\\right],\n",
    "\\end{cases}\n",
    "$$\n",
    "\n",
    "where $p^2=|f_1|^2= p^2_x+p^2_y$, and we have used $\\mu = \\mu_1 + \\mu_\\rho \\rho$."
   ]
  },
  {
   "cell_type": "markdown",
   "metadata": {},
   "source": [
    "### Derivation\n",
    "Expanding $f$ in angular Fourier modes ($f_k(\\mathbf{r}, t)=\\frac{1}{2\\pi}\\sum_k f(\\mathbf{r}, \\theta, t) \\exp (-ik\\theta)$) leads to the hierachy\n",
    "$$\\partial_t f_k + \\frac{1}{2} (\\nabla^*f_{k+1} +\\nabla f_{k-1}) = (P_k - 1)f_k + \\rho_0 \\sum_q J_{k, q} f_q f_{k-q},$$\n",
    "For $k=0$, noting that $J_{0, q}=0$ ant $P_0 = 1$, we have\n",
    "$$\\partial_t f_0 = -\\frac{1}{2} (\\nabla^* f_1 + \\nabla f_{-1})=-\\Re(\\nabla^* f_1)$$\n",
    "\n",
    "For $k=1$, keeping in mind that $|q|+|1-q| \\le 3$, i.e., $q=-1, 0, 1, 2$, thus\n",
    "\n",
    "$$\n",
    "\\begin{aligned}\n",
    "\\sum_q J_{1, q}f_q f_{1-q}&=J_{1, -1}f_{-1}f_{2}+J_{1, 0}f_0 f_1 + J_{1, 1} f_1 f_0 + J_{1, 2}f_2 f_{-1}  \\\\\n",
    "&= (J_{1, -1}+J_{1, 2})f_{-1}f_2+(J_{1, 0}+J_{1, 1})f_0 f_1,\n",
    "\\end{aligned}\n",
    "$$\n",
    "\n",
    "Then $f_1$ can be expressed as:\n",
    "$$\n",
    "\\begin{aligned}\n",
    "\\partial_t f_1 + \\frac{1}{2} (\\nabla^* f_2 + \\nabla f_0)&=(P_1 - 1)f_1 + \\rho_0 (J_{1, -1}+J_{1, 2})f_{-1}f_2 + \\rho_0 (J_{1, 0}+J_{1, 1})f_0 f_1 \\\\\n",
    "&= \\mu f_1 + \\rho_0 (J_{1, -1}+J_{1, 2})f^*_1 f_2,\n",
    "\\end{aligned}\n",
    "$$\n",
    "where $\\mu = P_1 - 1 + \\rho_0 (J_{1, 0}+J_{1, 1})f_0$\n",
    "For $k=2$, to satisfy $|q|+|2-q| \\le 3$, $q$ should be $0, 1, 2$, so\n",
    "$$\\sum_q J_{2, q} f_q f_{2-q} = (J_{2, 0}+J_{2, 2})f_0 f_2 + J_{2, 1} f_1^2.$$\n",
    "Letting $\\partial_t f_2 = 0$ and $\\nabla^* f_3 = 0$, one gets\n",
    "$$\\frac{1}{2} \\nabla f_1=(P_2 - 1) f_2 + \\rho_0 (J_{2, 0}+J_{2, 2})f_0 f_2 + \\rho_0 J_{2, 1} f_1^2,$$\n",
    "Denoting $\\mu_2 = (P_2 - 1) + \\rho_0 f_0 (J_{2, 0} + J_{2, 2})$, the above equation can be expressed as\n",
    "$$f_2 = \\frac{1}{2\\mu_2} \\nabla f_1 - \\frac{\\rho_0 J_{2, 1}}{\\mu_2} f_1^2,$$\n",
    "\n",
    "Once the expression of $f_2$ is obtained, $f_1$ can be expressed as\n",
    "\n",
    "$$\n",
    "\\begin{aligned}\n",
    "\\partial_t f_1 &= -\\frac{1}{2}\\nabla f_0 + \\mu f_1- \\frac{1}{2} \\nabla^* f_2  + \\rho_0 (J_{1, -1}+J_{1, 2})f^*_1 f_2\\\\\n",
    "&=-\\frac{1}{2}\\nabla f_0 + \\mu f_1 -\\frac{1}{2} \\nabla^* (\\frac{1}{2\\mu_2} \\nabla f_1 - \\frac{\\rho_0 J_{2, 1}}{\\mu_2} f_1^2) + \\rho_0 (J_{1, -1}+J_{1, 2})f^*_1 (\\frac{1}{2\\mu_2} \\nabla f_1 - \\frac{\\rho_0 J_{2, 1}}{\\mu_2} f_1^2)\\\\\n",
    "&=-\\frac{1}{2}\\nabla f_0 + (\\mu - \\xi |f_1|^2) f_1 + \\kappa_1 f^*_1 \\nabla f_1 -\\frac{1}{2} \\nabla^* (\\frac{1}{2\\mu_2} \\nabla f_1 - \\frac{\\rho_0 J_{2, 1}}{\\mu_2} f_1^2),\n",
    "\\end{aligned}\n",
    "$$\n",
    "\n",
    "where $\\xi = \\frac{\\rho^2_0 (J_{1, -1} + J_{1, 2})J_{2, 1}}{\\mu_2}$ and $\\kappa_1 = \\frac{\\rho_0(J_{1, -1} + J_{1, 2})}{2\\mu_2}$.\n",
    "\n",
    "If both $\\mu_2$ and $J_{2, 1}$ are independent of $\\mathbf{r}$, the expression of $f_1$ can be further simplified as\n",
    "$$\\partial_tf_1 = -\\frac{1}{2}\\nabla f_0 + (\\mu - \\xi |f_1|^2) f_1 + \\kappa_1 f^*_1 \\nabla f_1 + \\kappa_2 \\nabla^* f_1^2 + \\nu \\Delta f_1,$$\n",
    "where $\\kappa_2 = \\frac{\\rho_0 J_{2, 1}}{2\\mu_2}$ and $\\nu = -\\frac{1}{4\\mu_2}$."
   ]
  }
 ],
 "metadata": {
  "kernelspec": {
   "display_name": "Python 3",
   "language": "python",
   "name": "python3"
  },
  "language_info": {
   "codemirror_mode": {
    "name": "ipython",
    "version": 3
   },
   "file_extension": ".py",
   "mimetype": "text/x-python",
   "name": "python",
   "nbconvert_exporter": "python",
   "pygments_lexer": "ipython3",
   "version": "3.7.0"
  }
 },
 "nbformat": 4,
 "nbformat_minor": 2
}
